pulse/src/syntax_extension/PulseDesugar.fst
@@ -71,12 +71,12 @@ let stt_lid = Ident.lid_of_path ["Pulse"; "Steel"; "Wrapper"; "stt"] r_
 let assign_lid = Ident.lid_of_path ["Pulse"; "Steel"; "Wrapper"; "write"] r_
 let stt_ghost_lid = Ident.lid_of_path ["Pulse"; "Steel"; "Wrapper"; "stt_ghost"] r_
 let stt_atomic_lid = Ident.lid_of_path ["Pulse"; "Steel"; "Wrapper"; "stt_atomic"] r_
-let stapp_assignment (lhs rhs:S.term) 
+let stapp_assignment (lhs rhs:S.term) (r:_)
   : SW.st_term
   = let head_fv = S.lid_as_fv assign_lid S.delta_equational None in
     let head = S.fv_to_tm head_fv in
     let app = S.mk_Tm_app head [(lhs, None)] lhs.pos in
-    SW.(tm_st_app (tm_expr app) None (as_term rhs))
+    SW.(tm_st_app (tm_expr app) None (as_term rhs) r)
 
 
 let resolve_name (env:env_t) (id:ident)
@@ -101,9 +101,10 @@ let pulse_arrow_formals (t:S.term) =
     )
     else None
 
-let stapp_or_return (env:env_t) (s:S.term) 
+let stapp_or_return (env:env_t) (s:S.term)
   : SW.st_term
-  = let ret s = SW.(tm_return (as_term s)) in
+  = let r = s.pos in
+    let ret s = SW.(tm_return (as_term s) r) in
     let head, args = U.head_and_args_full s in
     match head.n with
     | S.Tm_fvar fv -> (
@@ -153,7 +154,7 @@ let stapp_or_return (env:env_t) (s:S.term)
             then ( //this is an st app
               let head = S.mk_Tm_app head (L.init args) s.pos in
               let last, q = L.last args in
-              SW.(tm_st_app (tm_expr head) q (as_term last))
+              SW.(tm_st_app (tm_expr head) q (as_term last) r)
             )
             else (
               //partial app of a stateful function
@@ -231,10 +232,10 @@ let rec desugar_vprop (env:env_t) (v:Sugar.vprop)
       in
       aux env binders
 
-let mk_bind b s1 s2 : SW.st_term = 
+let mk_bind b s1 s2 r : SW.st_term = 
   if SW.is_tm_intro_exists s1
-  then SW.tm_bind b (SW.tm_protect s1) (SW.tm_protect s2)
-  else SW.tm_bind b s1 s2
+  then SW.tm_bind b (SW.tm_protect s1) (SW.tm_protect s2) r
+  else SW.tm_bind b s1 s2 r
 
 (* s has already been transformed with explicit dereferences for r-values *)
 let rec desugar_stmt (env:env_t) (s:Sugar.stmt)
@@ -249,17 +250,17 @@ let rec desugar_stmt (env:env_t) (s:Sugar.stmt)
     | Assignment { id; value } ->
       let? lhs = resolve_name env id in
       let? value = tosyntax env value in
-      return (stapp_assignment lhs value)
-
+      return (stapp_assignment lhs value s.range)
+    
     | Sequence { s1={s=Open l}; s2 } ->
       let env = push_namespace env l in
       desugar_stmt env s2
 
     | Sequence { s1={s=LetBinding lb}; s2 } ->
-      desugar_bind env lb s2
+      desugar_bind env lb s2 s.range
 
     | Sequence { s1; s2 } -> 
-      desugar_sequence env s1 s2
+      desugar_sequence env s1 s2 s.range
       
     | Block { stmt } ->
       desugar_stmt env stmt
@@ -277,11 +278,11 @@ let rec desugar_stmt (env:env_t) (s:Sugar.stmt)
       let? else_ = 
         match else_opt with
         | None -> 
-          return (tm_return (tm_expr S.unit_const))
+          return (tm_return (tm_expr S.unit_const) R.dummyRange)
         | Some e -> 
           desugar_stmt env e
       in
-      return (SW.tm_if head join_vprop then_ else_)
+      return (SW.tm_if head join_vprop then_ else_ s.range)
 
     | Match { head; returns_annot; branches } ->
       failwith "Match is not yet handled"
@@ -294,7 +295,7 @@ let rec desugar_stmt (env:env_t) (s:Sugar.stmt)
         return (SW.close_term inv bv.index)
       in
       let? body = desugar_stmt env body in
-      return (SW.tm_while guard (id, invariant) body)
+      return (SW.tm_while guard (id, invariant) body s.range)
 
     | Introduce { vprop; witnesses } -> (
       match vprop with
@@ -303,7 +304,7 @@ let rec desugar_stmt (env:env_t) (s:Sugar.stmt)
       | VPropExists _ ->
         let? vp = desugar_vprop env vprop in
         let? witnesses = map_err (desugar_term env) witnesses in
-        return (SW.tm_intro_exists false vp witnesses)
+        return (SW.tm_intro_exists false vp witnesses s.range)
     )
 
 
@@ -314,17 +315,17 @@ let rec desugar_stmt (env:env_t) (s:Sugar.stmt)
       let? q2 = desugar_vprop env q2 in      
       let? b1 = desugar_stmt env b1 in
       let? b2 = desugar_stmt env b2 in
-      return (SW.tm_par p1 p2 q1 q2 b1 b2)
+      return (SW.tm_par p1 p2 q1 q2 b1 b2 s.range)
 
     | Rewrite { p1; p2 } ->
       let? p1 = desugar_vprop env p1 in
       let? p2 = desugar_vprop env p2 in
-      return (SW.tm_rewrite p1 p2)
+      return (SW.tm_rewrite p1 p2 s.range)
 
     | LetBinding _ -> 
       fail "Terminal let binding" s.range
 
-and desugar_bind (env:env_t) (lb:_) (s2:Sugar.stmt) 
+and desugar_bind (env:env_t) (lb:_) (s2:Sugar.stmt) (r:R.range)
   : err SW.st_term
   = let open Sugar in
     let? annot = desugar_term_opt env lb.typ in
@@ -342,20 +343,20 @@ and desugar_bind (env:env_t) (lb:_) (s2:Sugar.stmt)
       | None -> //just a regular bind
         let? s1 = tosyntax env e1 in
         let s1 = stapp_or_return env s1 in
-        return (mk_bind (SW.mk_binder lb.id annot) s1 s2)
+        return (mk_bind (SW.mk_binder lb.id annot) s1 s2 r)
       
       | Some MUT //these are handled the same for now
       | Some REF -> 
         let? e1 = desugar_term env e1 in 
-        return (SW.tm_let_mut lb.id annot e1 s2)
+        return (SW.tm_let_mut lb.id annot e1 s2 r)
     )
 
-and desugar_sequence (env:env_t) (s1 s2:Sugar.stmt)
+and desugar_sequence (env:env_t) (s1 s2:Sugar.stmt) r
   : err SW.st_term
   = let? s1 = desugar_stmt env s1 in
     let? s2 = desugar_stmt env s2 in
     let annot = SW.mk_binder (Ident.id_of_text "_") SW.tm_unknown in
-    return (mk_bind annot s1 s2)
+    return (mk_bind annot s1 s2 r)
 
 let explicit_rvalues (env:env_t) (s:Sugar.stmt)
   : Sugar.stmt
@@ -415,11 +416,15 @@ let desugar_decl (env:env_t)
       | [(q, last)], [last_bv] -> 
         let body = SW.close_st_term body last_bv.S.index in
         let comp = SW.close_comp comp last_bv.S.index in
-        return (SW.tm_abs last q (SW.comp_pre comp) body (Some (SW.comp_post comp)))
+        return (SW.tm_abs last q
+                          (SW.comp_pre comp)
+                          body
+                          (Some (SW.comp_post comp))
+                          p.range)
       | (q, b)::bs, bv::bvs ->
         let? body = aux bs bvs in
         let body = SW.close_st_term body bv.index in
-        return (SW.tm_abs b q SW.tm_emp body None)
+        return (SW.tm_abs b q SW.tm_emp body None p.range)
       | _ -> fail "Unexpected empty binders in decl" r_
     in
     aux bs bvs
