pulse/lib/steel/pulse/Pulse.Syntax.Builder.fst
@@ -1,0 +1,18 @@
+module Pulse.Syntax.Builder
+open Pulse.Syntax
+
+let tm_return ctag insert_eq term = Tm_Return { ctag; insert_eq; term }
+let tm_abs b q pre body post = Tm_Abs { b; q; pre; body; post }
+let tm_stapp head arg_qual arg = Tm_STApp { head; arg_qual; arg }
+let tm_bind binder head body = Tm_Bind { binder; head; body }
+let tm_totbind head body = Tm_TotBind { head; body }
+let tm_if b then_ else_ post = Tm_If { b; then_; else_; post }
+let tm_elim_exists p = Tm_ElimExists { p }
+let tm_intro_exists erased p witnesses = Tm_IntroExists { erased; p; witnesses }
+let tm_while invariant condition body = Tm_While { invariant; condition; body }
+let tm_par pre1 body1 post1 pre2 body2 post2 = Tm_Par { pre1; body1; post1; pre2; body2; post2 }
+let tm_with_local initializer body = Tm_WithLocal { initializer; body }
+let tm_rewrite t1 t2 = Tm_Rewrite { t1; t2 }
+let tm_admit ctag u typ post = Tm_Admit { ctag; u; typ; post }
+let tm_protect t = Tm_Protect { t }
+let with_range t r = { term = t; range = r}
