pulse/src/syntax_extension/PulseSyntaxWrapper.fsti
@@ -11,20 +11,20 @@ val u_var (s:string) : universe
 val u_max (u0 u1:universe) : universe
 val u_unknown : universe
 
-val bv : Type0
+new val bv : Type0
 val mk_bv (i:index) (name:string) (r:range) : bv
 
-val nm : Type0
+new val nm : Type0
 val mk_nm (i:index) (name:string) (r:range) : nm
 
-val fv : Type0
+new val fv : Type0
 val mk_fv (nm:lident) (r:range) : fv
 
-val qualifier : Type0
+new val qualifier : Type0
 val as_qual (imp:bool) : option qualifier
-val term : Type0
-val binder : Type0
-val comp : Type0
+new val term : Type0
+new val binder : Type0
+new val comp : Type0
 let vprop = term
 val mk_binder (x:ident) (t:term) : binder
 
@@ -43,19 +43,19 @@ val mk_comp (pre:term) (ret:binder) (post:term) : comp
 val ghost_comp (inames:term) (pre:term) (ret:binder) (post:term) : comp
 val atomic_comp (inames:term) (pre:term) (ret:binder) (post:term) : comp
 
-val st_term : Type0
-val tm_return (t:term) : st_term
-val tm_abs (b:binder) (q:option qualifier) (pre:term) (body:st_term) (post:option term) : st_term
-val tm_st_app (head:term) (q:FStar.Syntax.Syntax.aqual) (arg:term) : st_term
-val tm_bind (x:binder) (e1:st_term) (e2:st_term) : st_term
-val tm_let_mut (x:ident) (t:term) (v:term) (k:st_term) : st_term
-val tm_while (head:st_term) (invariant: (ident & vprop)) (body:st_term) : st_term 
-val tm_if (head:term) (returns_annot:option vprop) (then_ else_:st_term) : st_term
-val tm_intro_exists (erased:bool) (vp:vprop) (witnesses:list term) : st_term
+new val st_term : Type0
+val tm_return (t:term) (_:range) : st_term
+val tm_abs (b:binder) (q:option qualifier) (pre:term) (body:st_term) (post:option term) (_:range) : st_term
+val tm_st_app (head:term) (q:FStar.Syntax.Syntax.aqual) (arg:term) (_:range) : st_term
+val tm_bind (x:binder) (e1:st_term) (e2:st_term) (_:range) : st_term
+val tm_let_mut (x:ident) (t:term) (v:term) (k:st_term) (_:range) : st_term
+val tm_while (head:st_term) (invariant: (ident & vprop)) (body:st_term) (_:range) : st_term 
+val tm_if (head:term) (returns_annot:option vprop) (then_ else_:st_term) (_:range) : st_term
+val tm_intro_exists (erased:bool) (vp:vprop) (witnesses:list term) (_:range) : st_term
 val is_tm_intro_exists (x:st_term) : bool
 val tm_protect (s:st_term) : st_term
-val tm_par (p1:term) (p2:term) (q1:term) (q2:term) (b1:st_term) (b2:st_term) : st_term
-val tm_rewrite (p1:term) (p2:term) : st_term
+val tm_par (p1:term) (p2:term) (q1:term) (q2:term) (b1:st_term) (b2:st_term) (_:range) : st_term
+val tm_rewrite (p1:term) (p2:term) (_:range) : st_term
 
 val close_term (t:term) (v:var) : term
 val close_st_term (t:st_term) (v:var) : st_term
